block_equiv_checker.v
@@ -1,5 +1,5 @@
 Require Import List.
-
+ 
 Require Import FORVES.program.
 Import Program.
 
