storage_cmp_impl_soundness.v
@@ -63,7 +63,46 @@ Module StorageCmpImplSoundness.
   Theorem basic_storage_cmp_snd:
     safe_sstorage_cmp_ext_wrt_sstack_value_cmp basic_storage_cmp.
   Proof.
-  Admitted.
+    Admitted.
+    (*
+    unfold safe_sstorage_cmp_ext_wrt_sstack_value_cmp.
+    intros d sstack_val_cmp H_sstack_val_cmp_snd.
+    unfold safe_sstorage_cmp_ext_d.
+    intros d' H_d'_le_d.
+    unfold safe_sstorage_cmp.
+    intros sstrg1 sstrg2 maxidx1 sb1 maxidx2 sb2 instk_height ops H_valid_sb1 H_valid_sb2.
+    revert sstrg2.
+    revert sstrg1.
+    induction sstrg1 as [|u1 sstrg1' IHsstrg1'].
+    + intros sstrg2 H_valid_sstrg1 H_valid_sstrg2 H_basic_strg_smp stk mem strg ctx.
+      destruct sstrg2; try discriminate.
+      exists strg.
+      unfold eval_sstorage.
+      simpl.
+      split; reflexivity.
+    + intros sstrg2 H_valid_sstrg1 H_valid_sstrg2 H_basic_strg_smp stk mem strg ctx.
+      destruct sstrg2 as [|u2 sstrg2'] eqn:H_sstrg2.
+      ++ simpl in H_basic_strg_smp.
+         destruct u1.
+         discriminate.
+      ++ simpl in H_basic_strg_smp.
+         destruct u1 as [skey1 svalue1] eqn:E_u1.
+         destruct u2 as [skey2 svalue2] eqn:E_u2.
+         destruct (sstack_val_cmp d' skey1 skey2 maxidx1 sb1 maxidx2 sb2 instk_height ops) eqn:E_cmp_skey1_skey2; try discriminate.
+         destruct (sstack_val_cmp d' svalue1 svalue2 maxidx1 sb1 maxidx2 sb2 instk_height ops) eqn:E_cmp_svalue1_svalue2; try discriminate.
+         simpl in H_valid_sstrg1.
+         destruct H_valid_sstrg1 as [ [H_valid_skey1 H_valid_svalue1] H_valid_sstrg1'].
+         simpl in H_valid_sstrg2.
+         destruct H_valid_sstrg2 as [ [H_valid_skey2 H_valid_svalue2] H_valid_sstrg2'].
+         pose proof (IHsstrg1' sstrg2' H_valid_sstrg1' H_valid_sstrg2' H_basic_strg_smp stk mem strg ctx) as IHsstrg1'_0.
+         destruct IHsstrg1'_0 as [strg' [IHsstrg1'_0 IHsstrg1'_1]].
+
+         unfold safe_sstack_val_cmp_ext_1_d in H_sstack_val_cmp_snd.
+         pose proof (H_sstack_val_cmp_snd d' H_d'_le_d) as H_sstack_val_cmp_snd_d'.
+         unfold safe_sstack_val_cmp in H_sstack_val_cmp_snd_d'.
+         pose proof(H_sstack_val_cmp_snd_d' skey1 skey2 maxidx1 sb1 maxidx2 sb2 instk_height ops H_valid_skey1 H_valid_skey2 H_valid_sb1 H_valid_sb2 E_cmp_skey1_skey2 stk mem strg ctx H_s).
+         pose proof (H_sstack_val_cmp_snd
+*)
   
   Theorem po_storage_cmp_snd:
     safe_sstorage_cmp_ext_wrt_sstack_value_cmp po_storage_cmp.
